Update refine

theories/os/refine.v
@@ -9,16 +9,16 @@ From iris_os.os Require Export spec refine_ra.
 Set Default Proof Using "Type".
 Import uPred.
 
+Instance equiv_cfg: Equiv cfg := (=).
+
+Definition specM := (prodR fracR (agreeR (discreteC cfg))).
+
 Class specG K Σ := SpecG {
-    specG_spstG :> gen_heapG ident val Σ;
-    specG_specG :> inG Σ (prodR fracR (agreeR (discreteC (spec_code))));
-    spec_gname : gname;
+    specG_cfgG :> inG Σ specM;
+    cfgG_gname : gname;
     refine_inG :> inG Σ (@refine_ucmra K);
     refine_gname : gname
 }.
-
-Notation "l S↦ v" :=
-  (@mapsto _ _ _ _ _ specG_spstG l 1%Qp v) (at level 20) : uPred_scope.
 
 Section specG.
   Context `{specG K Σ}.
@@ -27,7 +27,11 @@ Section specG.
 
   Definition master_own_exact cs := own refine_gname (refine master cs).
 
+  Definition master_own c := (∃ cs, own refine_gname (refine master (c :: cs)))%I.
+
   Definition snapshot_own_exact cs := own refine_gname (refine snapshot cs).
+
+  Definition snapshot_own c := (∃ cs, own refine_gname (refine snapshot (c :: cs)))%I.
 
   Lemma valid_refine_op cs1 cs2:
     ✓ (refine master cs1 ⋅ refine snapshot cs2) →
@@ -48,7 +52,16 @@ Section specG.
     - simpl. split; [|split]=>//. apply refine_disj'.
   Qed.
 
-  Lemma spec_grow:
+  Lemma refine_snap:
+    ∀ c,
+      master_own c ⊢ |==> master_own c ∗ snapshot_own c.
+  Proof.
+    iIntros (c) "Hm". iDestruct "Hm" as (cs) "Hm".
+    iMod (refine_snap' with "Hm") as "[Hm Hs]".
+    iSplitL "Hm"; by iExists _.
+  Qed.
+
+  Lemma master_grow':
     ∀ c0 c cs,
       spec_step' c0 c →
       master_own_exact (c0::cs) ⊢ |==> master_own_exact (c::c0::cs).
@@ -65,48 +78,42 @@ Section specG.
     - simpl. constructor=>//.
   Qed.
 
-  Definition γ_sstate := @gen_heap_name _ _ _ _ _ specG_spstG.
+  Lemma master_grow:
+    ∀ c c',
+      spec_step' c c' →
+      master_own c ⊢ |==> master_own c'.
+  Proof.
+    iIntros (???) "Ho".
+    iDestruct "Ho" as (?) "Ho".
+    iExists _. iApply master_grow'=>//.
+  Qed.
 
-  Definition sstate (s: spec_state) := ([⋅ map] l ↦ v ∈ s, l S↦ v)%I.
-  Definition scode (c: spec_code) := own spec_gname ((1/2)%Qp, (to_agree (c: leibnizC spec_code))).
+  Definition to_cfgM (c: cfg) : specM :=
+    ((1/2)%Qp, (to_agree (c: leibnizC cfg))).
+  
+  Definition own_cfg (c: cfg) := own cfgG_gname (to_cfgM c).
 
-  Lemma mapsto_singleton l v:
-    l S↦ v ⊣⊢ sstate {[ l := v ]}.
-  Proof. by rewrite /sstate big_sepM_singleton. Qed.
-
-  Definition spec_inv :=
-    (∃ c0 s0 c s cs,
-       scode c ∗ own γ_sstate (● to_gen_heap s) ∗
-       master_own_exact ((s, c)::cs) ∗ ⌜ spec_step_star c0 s0 c s ⌝)%I.
+  Definition spec_inv := (∃ c, own_cfg c ∗ master_own c)%I.
 
   Global Instance spec_inv_timeless: TimelessP spec_inv. Proof. apply _. Qed.
-
-  Lemma sstate_update s ss ss':
-    own γ_sstate (● to_gen_heap s) ∗
-    ([∗ map] l↦v ∈ ss, l S↦ v)
-    ⊢ (∃ s', own γ_sstate (● to_gen_heap s') ∗
-             ([∗ map] l↦v ∈ ss', l S↦ v) ∗
-             ⌜ ∃ sf, gset_dom sf ⊥ gset_dom ss ∧ s = sf ∪ ss ∧ s' = sf ∪ ss' ⌝).
-  Proof.
-  Admitted.
-
-  Lemma scode_agree ks ks':
-   scode ks ∗ scode ks'  ⊢ ⌜ ks = ks' ⌝.
+  
+  Lemma own_cfg_agree ks ks':
+   own_cfg ks ∗ own_cfg ks'  ⊢ ⌜ ks = ks' ⌝.
   Proof.
     iIntros "[Hs' Hs]".
-    rewrite /scode.
+    rewrite /own_cfg.
     iDestruct (own_valid_2 with "Hs Hs'") as "%".
     iPureIntro. destruct H0 as [? ?]. simpl in H1.
     by apply to_agree_comp_valid in H1.
   Qed.
 
-  Lemma scode_update c1 c2 c3:
-    scode c1 ∗ scode c2 ⊢ |==> scode c3 ∗ scode c3 ∗ ⌜ c1 = c2 ⌝.
+  Lemma own_cfg_update c1 c2 c3:
+    own_cfg c1 ∗ own_cfg c2 ⊢ |==> own_cfg c3 ∗ own_cfg c3 ∗ ⌜ c1 = c2 ⌝.
   Proof.
     iIntros "[Hs Hs']".
-    iDestruct (scode_agree with "[-]") as "%"; first iFrame.
+    iDestruct (own_cfg_agree with "[-]") as "%"; first iFrame.
     inversion H0. subst.
-    rewrite /scode.
+    rewrite /own_cfg.
     iMod (own_update_2 with "Hs Hs'") as "[Hs Hs']"; last by iFrame.
     rewrite pair_op frac_op' Qp_div_2.
     apply cmra_update_exclusive.
@@ -115,31 +122,18 @@ Section specG.
     - by apply to_agree_comp_valid.
   Qed.
 
-  Lemma spec_update {sc sc'} ss ss':
-    spec_step sc ss sc' ss' →
-    spec_inv ∗ sstate ss ∗ scode sc
-    ⊢ |==> (∃ cs, spec_inv ∗ sstate ss' ∗ scode sc' ∗ snapshot_own_exact ((ss', sc')::(ss, sc)::cs)).
+  Lemma spec_update c c':
+    spec_step' c c' →
+    spec_inv ∗ own_cfg c ∗ snapshot_own c
+    ⊢ |==> spec_inv ∗ own_cfg c' ∗ snapshot_own c'.
   Proof.
-    (* iIntros (?) "(Hinv & Hss & Hsc)". *)
-    (* iDestruct "Hinv" as (c0 s0 c s) "(HSC & HSS & %)". *)
-    (* rewrite /sstate /scode. *)
-    (* (* HSC Hsc and sc' are easy to prove *) *)
-    (* (* ss, s => ss' are hard, might need some framing properties *) *)
-    (* iDestruct (sstate_update s ss ss' with "[HSS Hss]") as (s') "(HSS' & Hss' & %)"; first iFrame. *)
-    (* iMod (scode_update _ _ sc' with "[HSC Hsc]") as "(HSC' & Hsc' & %)"; first iFrame. *)
-    (* iSplitL "HSS' HSC'". *)
-    (* { iExists c0, s0, sc', s'. iFrame. *)
-    (*   destruct H2 as (sf & ? & ? & ?). *)
-    (*   subst. iPureIntro. *)
-    (*   eapply SStrans=>//. *)
-    (*   apply spec_step_framing=>//. *)
-    (* } *)
-    (* by iFrame. *)
-  Admitted.
-
-  Lemma spec_recover ss sc cs ss0 sc0:
-    spec_inv ∗ sstate ss ∗ scode sc ∗ snapshot_own_exact ((ss0, sc0)::cs)
-    ⊢ ⌜ spec_step_star sc0 ss0 sc ss ⌝.
-  Admitted.
-
+    iIntros (?) "(Hinv & Hc & _)".
+    iDestruct "Hinv" as (c'') "(HC & Hm)".
+    iMod (own_cfg_update _ _ c' with "[HC Hc]") as "(HC' & Hc' & %)"; first iFrame.
+    iFrame. subst.
+    iMod (master_grow _ c' with "Hm") as "Hm'"=>//.
+    iMod (refine_snap with "Hm'") as "[Hm' Hs']".
+    iFrame. iExists _. by iFrame.
+  Qed.
+  
 End specG.
